Update for camera-ready

Launchbury.v
@@ -34,19 +34,21 @@ CoInductive diverge_need : seq (option term) -> term -> Prop :=
       diverge_need (H ++ map (@Some _ \o subst s) ts) (subst s t) ->
       diverge_need H (Let ts t).
 
-Definition corr_heap_segment (f f' : nat -> nat -> Prop) H1 H2 :=
-  forall l1 l2, f l1 l2 ->
+Definition corr_heap_segment (R R' : nat -> nat -> Prop) H1 H2 :=
+  forall l1 l2, R l1 l2 ->
   exists t1, nth None H1 l1 = Some t1 /\
   exists t2, nth None H2 l2 = Some t2 /\
-  ( corr_term f' t1 t2 \/
-    wf_term (fun l => exists l', f' l l') t1 /\
-    exists H1' v1,
-    eval_name H1 t1 H1' v1 /\
-    exists g,
-    iso_heap g H1' H1 /\
-    corr_term (fun l0 l2 => exists l1, g l0 l1 /\ f' l1 l2) v1 t2 ).
+  ( corr_term R' t1 t2 \/
+    exists H2' v2,
+    eval_name H2 t2 H2' v2 /\
+    exists S,
+    iso_heap S H2 H2' /\
+    corr_term (fun l0 l2 => R' l0 l2 \/ exists l1, R' l0 l1 /\ S l1 l2) t1 v2 /\
+    forall l2', R l1 l2' ->
+    exists t2', nth None H2 l2' = Some t2' /\
+    corr_term (fun l2 l2' => exists l1, R' l1 l2 /\ R' l1 l2') t2 t2' ).
 
-Definition corr_heap f := corr_heap_segment f f.
+Definition corr_heap R := corr_heap_segment R R.
 
 Hint Constructors eval_need.
 
@@ -98,19 +100,6 @@ Proof.
   repeat eexists. eauto.
 Qed.
 
-Corollary corr_heap_segemtn_refl p p' H :
-  wf_heap_segment p p' H ->
-  corr_heap_segment
-    (fun l l' => l = l' /\ p l)
-    (fun l l' => l = l' /\ p' l) H H.
-Proof. by move => /iso_heap_segment_refl /iso_heap_segment_corr_heap_segment. Qed.
-
-Lemma corr_heap_segment_union fdom fdom' fcod H1 H2 :
-  corr_heap_segment fdom fcod H1 H2 ->
-  corr_heap_segment fdom' fcod H1 H2 ->
-  corr_heap_segment (fun l l' => fdom l l' \/ fdom' l l') fcod H1 H2.
-Proof. by move => Hcorr Hcorr' ? ? [ /Hcorr | /Hcorr' ]. Qed.
-
 Lemma corr_heap_segment_boundL f f' H H' :
   corr_heap_segment f f' H H' ->
   forall l l', f l l' ->
@@ -133,491 +122,232 @@ Lemma corr_heap_segment_wf_heap_segmentL f f' H H' :
   corr_heap_segment f f' H H' ->
   wf_heap_segment (fun l => exists l', f l l') (fun l => exists l', f' l l') H.
 Proof.
-  move => Hcorr ? [ ? /Hcorr [ ? [ -> [ ? [ ? [ | [ ] ] ] ] ] ] ];
-  eauto using corr_term_wf_termL.
+  move => Hcorr ? [ ? /Hcorr
+    [ ? [ -> [ ? [ ? [ ? | [ ? [ ? [ ? [ ? [ ? [ ? ? ] ] ] ] ] ] ] ] ] ] ] ];
+  repeat (eexists; eauto).
+  - apply: corr_term_wf_termL. eauto.
+  - apply: wf_term_impl.
+    + apply: corr_term_wf_termL. eauto.
+    + move => ? [ ? [ | [ ? [ ] ] ] ]; eauto.
 Qed.
 
-Lemma corr_heap_segment_wf_heap_segmentR f f' H H' :
+Lemma corr_heap_segment_iso_heap_segmentR R R' H1 H2 :
+  corr_heap_segment R R' H1 H2 ->
+  iso_heap_segment
+    (fun l2 l2' => exists l1, R l1 l2 /\ R l1 l2')
+    (fun l2 l2' => exists l1, R' l1 l2 /\ R' l1 l2') H2 H2.
+Proof.
+  move => Hcorr ? ? [ ? [ HR HR' ] ];
+  move: (Hcorr _ _ HR) =>
+    [ ? [ Hnth1 [ ? [ Hnth2 [ ? | [ ? [ ? [ ? [ ? [ ? [ ? ? ] ] ] ] ] ] ] ] ] ] ];
+  rewrite Hnth2; eauto.
+  move: (Hcorr _ _ HR') =>
+    [ ? [ Hnth1' [ ? [ Hnth2' [ ? | [ ? [ ? [ ? [ ? [ ? [ ? Hcon' ] ] ] ] ] ] ] ] ] ] ];
+  move: (Hnth2') Hnth1 Hnth1' => -> ->; inversion 1; subst;
+  repeat (eexists; eauto).
+  - apply: corr_term_comp; eauto.
+    exact: corr_term_sym.
+  - move: Hnth2 (Hcon' _ HR) => -> [ ? [ ] ].
+    inversion 1. subst => [ /corr_term_sym /corr_term_impl ].
+    apply => ? ? [ ? [ ] ]. eauto.
+Qed.
+
+Corollary corr_heap_segment_wf_heap_segmentR f f' H H' :
   corr_heap_segment f f' H H' ->
   wf_heap_segment (fun l' => exists l, f l l') (fun l' => exists l, f' l l') H'.
 Proof.
-  move => Hcorr ? [ ? /Hcorr [ ? [ ? [ ? [ -> [ ? | [ ? [ ? [ ? [ ? [ ? [ ? ? ] ] ] ] ] ] ] ] ] ] ] ];
-  repeat eexists; (apply: wf_term_impl; [ apply: corr_term_wf_termR | ]); eauto.
-  move => ? [ ? [ ? [ ] ] ]. eauto.
+  move => /corr_heap_segment_iso_heap_segmentR /iso_heap_segment_wf_heap_segmentL Hwf.
+  apply: wf_heap_segment_dom.
+  - apply: wf_heap_segment_cod; eauto.
+    move => ? [ ? [ ? [ ] ] ]. eauto.
+  - move => ? [ ]. eauto.
 Qed.
 
 Lemma corr_heap_segment_dom (fdom fdom' fcod : nat -> nat -> Prop) H H' :
   corr_heap_segment fdom fcod H H' ->
   (forall l l', fdom' l l' -> fdom l l') ->
   corr_heap_segment fdom' fcod H H'.
-Proof. by move => Hcorr Hdom ? ? /Hdom /Hcorr. Qed.
+Proof.
+  move => Hcorr Hdom ? ? /Hdom /Hcorr
+    [ ? [ -> [ ? [ -> [ ? | [ ? [ ? [ ? [ ? [ ? [ ? ? ] ] ] ] ] ] ] ] ] ] ];
+  repeat (repeat (eexists; eauto); right).
+Qed.
 
 Lemma corr_heap_segment_cod (fdom fcod fcod' : nat -> nat -> Prop) H H' :
   corr_heap_segment fdom fcod H H' ->
   (forall l l', fcod l l' -> fcod' l l') ->
   corr_heap_segment fdom fcod' H H'.
 Proof.
-  move => Hcorr Hcod ? ? /Hcorr [ ? [ -> [ ? [ -> [ ? | [ ? [ ? [ ? [ ? [ ? [ ? ? ] ] ] ] ] ] ] ] ] ] ];
-  repeat eexists.
-  - eauto using corr_term_impl.
-  - right. split.
-    + apply: wf_term_impl; eauto.
-      move => ? [ ]. eauto.
-    + repeat (eexists; eauto).
-      apply: corr_term_impl; eauto.
-      move => ? ? [ ? [ ] ]. eauto.
-Qed.
-
-Lemma corr_heap_segment_extR fdom fcod H1 H2 H2' :
-  corr_heap_segment fdom fcod H1 H2 ->
-  ( forall l l', fdom l l' ->
-    forall t,
-    nth None H2 l' = Some t ->
-    nth None H2' l' = Some t ) ->
-  corr_heap_segment fdom fcod H1 H2'.
-Proof.
-  move => Hcorr Hext ? ? Hf.
-  move: (Hcorr _ _ Hf) =>
-    [ ? [ -> [ ? [ /(Hext _ _ Hf) -> ] ] ] ] 
-    [ ? | [ ? [ ? [ ? [ ? [ ? [ ? ? ] ] ] ] ] ] ];
+  move => Hcorr Hcod ? ? /Hcorr
+    [ ? [ -> [ ? [ -> [ ? | [ ? [ ? [ ? [ ? [ ? [ ? Hcon ] ] ] ] ] ] ] ] ] ] ];
   repeat (eexists; eauto).
-  right. repeat (eexists; eauto).
+  - eauto using corr_term_impl.
+  - right. do 6 (eexists; eauto).
+    { apply: corr_term_impl; eauto.
+      move => ? ? [ | [ ? [ ] ] ]; eauto. }
+    move => ? /Hcon [ ? [ -> ? ] ].
+    repeat (eexists; eauto).
+    apply: corr_term_impl; eauto.
+    move => ? ? [ ? [ ] ]. eauto.
 Qed.
 
-Corollary corr_heap_segment_catR fdom fcod H1 H2 Hd :
-  corr_heap_segment fdom fcod H1 H2 ->
-  corr_heap_segment fdom fcod H1 (H2 ++ Hd).
-Proof.
-  move => /corr_heap_segment_extR.
-  apply => ? l' ? ?.
-  by move: nth_cat (leqP (size H2) l') => -> [ /(nth_default _) -> | ].
-Qed.
-
-Corollary corr_heap_segment_rconsR fdom fcod H1 H2 o :
-  corr_heap_segment fdom fcod H1 H2 ->
-  corr_heap_segment fdom fcod H1 (rcons H2 o).
-Proof. by rewrite -cats1 => /corr_heap_segment_catR. Qed.
-
-Lemma iso_heap_corr_heap_segment_comp (f fdom fcod : nat -> nat -> Prop) H H' H'' :
-  iso_heap f H H' ->
-  (forall l' l'', fcod l' l'' -> f l' l') ->
-  corr_heap_segment fdom fcod H' H'' ->
-  corr_heap_segment
-    (fun l l'' => exists l', f l l' /\ fdom l' l'')
-    (fun l l'' => exists l', f l l' /\ fcod l' l'') H H''.
-Proof.
-  move => Hiso Hsur Hcorr ? ? [ ? [ ] ] /Hiso [ ? [ -> [ ? [ Hnth Hterm ] ] ] ]
-    /Hcorr [ ? [ Hnth' [ ? [ -> [ Hterm' | [ ? [ ? [ ? [ Hcbn [ ? [ Hiso' Hterm' ] ] ] ] ] ] ] ] ] ] ];
-  move: Hnth Hnth' => ->; inversion 1; subst;
-  repeat eexists.
-  - eauto using corr_term_comp.
-  - right. split.
-    + apply: wf_term_impl.
-      { apply: corr_term_wf_termL.
-        apply: corr_term_comp; eauto.
-        apply: corr_term_refl. eauto. }
-      move => ? [ ? [ ? [ ? [ ? [ ] ] ] ] ]. subst. eauto.
-    + move: (eval_name_iso_heap _ _ _ _ Hcbn _ _ _ Hterm Hiso) =>
-        [ ? [ ? [ ? [ ? [ ? [ ? ? ] ] ] ] ] ].
-      { do 5 (eexists; eauto).
-        - apply: iso_heap_segment_comp; eauto.
-          apply: iso_heap_segment_comp; eauto.
-          apply: iso_heap_segment_sym. eauto.
-        - apply: corr_term_impl.
-          + apply: corr_term_comp; eauto.
-          + move => ? ? [ ? [ ? [ ? [ ? ? ] ] ] ].
-            repeat (eexists; eauto). }
-Qed.
-
-Corollary corr_heap_extL f H1 H1' H2 :
-  corr_heap f H1 H2 ->
-  ( forall l l', f l l' ->
+Lemma corr_heap_segment_extL R R' H1 H1' H2 :
+  corr_heap_segment R R' H1 H2 ->
+  ( forall l l', R l l' ->
     forall t,
     nth None H1 l = Some t ->
     nth None H1' l = Some t ) ->
-  corr_heap f H1' H2.
+  corr_heap_segment R R' H1' H2.
 Proof.
-  move => Hcorr Hext.
-  apply: corr_heap_segment_dom.
-  - apply: corr_heap_segment_cod.
-    + apply: iso_heap_corr_heap_segment_comp; eauto.
-      * { apply: iso_heap_segment_extL.
-          - apply: iso_heap_segment_refl.
-            apply: corr_heap_segment_wf_heap_segmentL; eauto.
-          - move => ? ? [ -> [ ] ]. eauto. }
-      * move => /=. eauto.
-    + by move => ? ? [ ? [ [ -> ] ] ].
-  - move => /=. eauto.
+  move => Hcorr Hext ? ? HR.
+  move: (Hcorr _ _ HR) =>
+    [ ? [ /(Hext _ _ HR) -> ] ]; eauto.
 Qed.
 
-Corollary corr_heap_catL f H1 H2 Hd :
-  corr_heap f H1 H2 ->
-  corr_heap f (H1 ++ Hd) H2.
+Corollary corr_heap_segment_catL fdom fcod H1 H2 Hd :
+  corr_heap_segment fdom fcod H1 H2 ->
+  corr_heap_segment fdom fcod (H1 ++ Hd) H2.
 Proof.
-  move => /corr_heap_extL.
+  move => /corr_heap_segment_extL.
   apply => l ? ? ?.
   by move: nth_cat (leqP (size H1) l) => -> [ /(nth_default _) -> | ].
 Qed.
 
-Corollary corr_heap_rconsL f H1 H2 o :
-  corr_heap f H1 H2 ->
-  corr_heap f (rcons H1 o) H2.
-Proof. by rewrite -cats1 => /corr_heap_catL. Qed.
+Corollary corr_heap_segment_rconsL fdom fcod H1 H2 o :
+  corr_heap_segment fdom fcod H1 H2 ->
+  corr_heap_segment fdom fcod (rcons H1 o) H2.
+Proof. by rewrite -cats1 => /corr_heap_segment_catL. Qed.
 
-Theorem eval_need_sound H2 t2 H2' v2 :
-  eval_need H2 t2 H2' v2 ->
-  forall f H1 t1,
-  corr_term f t1 t2 ->
-  corr_heap f H1 H2 ->
-  iso_heap (fun l1 l1' => exists l2, f l1 l2 /\ f l1' l2) H1 H1 ->
-  exists f' H1' v1,
-  eval_name H1 t1 H1' v1 /\
-  corr_heap f' H1' H2' /\
-  iso_heap (fun l1 l1' => exists l2, f' l1 l2 /\ f' l1' l2) H1' H1' /\
-  corr_term f' v1 v2 /\
-  (forall l1 l2, f l1 l2 -> f' l1 l2).
+Lemma corr_heap_segment_union fdom fdom' fcod H1 H2 :
+  corr_heap_segment fdom fcod H1 H2 ->
+  corr_heap_segment fdom' fcod H1 H2 ->
+  (forall l1 l2, fdom l1 l2 -> forall l2', fdom' l1 l2' -> False) ->
+  corr_heap_segment (fun l l' => fdom l l' \/ fdom' l l') fcod H1 H2.
 Proof.
-  induction 1; inversion 1; subst => [ Hcorr Hiso ].
-  - move: (Hcorr _ _ H6) => [ ? [ Hnth [ ? [ ] ] ] ].
-    rewrite H0. inversion 1.
-    subst => [ [ Hterm | [ ? [ H1' [ ? [ Hcbn [ g [ ? Hterm' ] ] ] ] ] ] ] ].
-    + move: (IHeval_need _ _ _ Hterm Hcorr Hiso) =>
-        [ f' [ ? [ ? [ Hcbn [ Hcorr' [ Hiso' [ ? Himpl ] ] ] ] ] ] ].
-      do 5 (eexists; eauto).
-      apply (corr_heap_segment_dom (fun l0 l' => l' != l /\ f' l0 l' \/ l' = l /\ f' l0 l')).
-      { apply: corr_heap_segment_union.
-        - apply: corr_heap_segment_extR.
-          + apply: corr_heap_segment_dom; eauto.
-            by move => ? ? [ ].
-          + move => ? ? [ /negPf Hneq ? ] ?.
-            rewrite nth_set_nth => /=.
-            by rewrite Hneq.
-        - move => ? ? [ ? ] Hf'. subst.
-          rewrite nth_set_nth => /=.
-          move: (Hiso' _ _ (ex_intro _ _ (conj Hf' (Himpl _ _ H6)))) =>
-            [ ? [ -> [ ? [ ] ] ] ].
-          rewrite (eval_name_heap _ _ _ _ Hcbn _ _ Hnth) eqxx.
-          inversion 1. subst => [ Hterm' ].
-          repeat eexists. right. split.
-          + apply: wf_term_impl.
-            * apply: corr_term_wf_termL; eauto.
-            * move => ? [ ? [ ? [ ] ] ]. eauto.
-          + move: (eval_name_iso_heap _ _ _ _ Hcbn _ _ _
-              (corr_term_comp _ _ _ _ Hterm' _
-                (corr_term_comp _ _ _ _ Hterm _ (corr_term_sym _ _ _ Hterm)))
-              (iso_heap_segment_comp _ _ _ _ _ _ _ Hiso'
-                (iso_heap_segment_extL _ _ _ _ _ Hiso
-                  (fun _ _ _ => eval_name_heap _ _ _ _ Hcbn _)))) =>
-              [ ? [ ? [ ? [ ? [ ? [ ? ? ] ] ] ] ] ].
-            repeat (eexists; eauto using corr_term_comp). }
-      move => ? l'.
-      case (@eqP _ l' l) => /= [ -> | ]; eauto.
-    + case: (eval_need_det _ _ _ _ H1 _ _
-        (value_eval_need _ _
-          (corr_term_valueL _ _ _ Hterm' (eval_name_value _ _ _ _ Hcbn)))) => ? ?. subst.
-      have Hiso' : iso_heap (fun l l' => g l l' \/ l = l' /\ exists l', f l l') H1' H2.
-      { apply: iso_heap_segment_union.
-        - apply: iso_heap_segment_cod; eauto.
-        - apply: iso_heap_segment_extL.
-          + apply: iso_heap_segment_cod.
-            * apply: iso_heap_segment_refl.
-              apply: corr_heap_segment_wf_heap_segmentL. eauto.
-            * eauto.
-          + move => ? ? ?. apply: eval_name_heap. eauto. }
-      do 5 (eexists; eauto).
-      { apply: (iso_heap_corr_heap_segment_comp _ f f _ _ _ Hiso'); eauto.
-        apply: (corr_heap_segment_extR _ _ _ _ _ Hcorr) => ? l' ? ?.
-        move: nth_set_nth (@eqP _ l' l) => -> /= [ ? | // ].
-        subst. by rewrite H0. }
-      split.
-      { apply: iso_heap_segment_dom.
-        - apply: iso_heap_segment_cod.
-          + apply: iso_heap_segment_comp; eauto.
-            apply: iso_heap_segment_sym.
-            apply: iso_heap_segment_comp; eauto.
-          + move => ? ?
-              [ ? [ ] ] [ ? | [ -> [ ? ? ] ] ]
-              [ ? [ ] ] [ ? | [ -> [ ? ? ] ] ] [ ? [ ? ? ] ];
-            repeat (eexists; eauto).
-        - move => ? ? [ ? [ ] ]
-            [ ? [ ] ] [ ? | [ -> [ ? ? ] ] ] ?
-            [ ? [ ] ] [ ? | [ -> [ ? ? ] ] ] ?;
-          repeat (rewrite -?plus_n_O; eexists; eauto). }
-      split.
-      { apply: corr_term_impl; eauto.
-        move => ? ? [ ? [ ] ]. eauto. }
-      eauto 6.
-  - move: (IHeval_need1 _ _ _ H7 Hcorr Hiso) =>
-      [ f' [ H1' [ ? [ ? [ Hcorr0 [ ? [ ] ] ] ] ] ] ].
-    inversion 1. subst => [ ? ].
-    have Hterm' : corr_term
-      (fun l l' => f' l l' \/ l = size H1' /\ l' = size H')
-      (subst (scons (Loc (size H1')) Var) t)
-      (subst (scons (Loc (size H')) Var) t0).
-    { apply: corr_term_subst => [ | [ | ? ] ] /=;
-      eauto using corr_term_impl. }
-    have Hcorr' : corr_heap
-      (fun l l' => f' l l' \/ l = size H1' /\ l' = size H')
-      (rcons H1' (Some t5)) (rcons H' (Some t2)).
-    { apply: corr_heap_segment_union.
-      - apply: corr_heap_segment_cod; eauto.
-        apply: corr_heap_rconsL.
-        by apply: corr_heap_segment_rconsR.
-      - apply: iso_heap_segment_corr_heap_segment => ? ? [ -> -> ].
-        rewrite !nth_rcons !ltnn !eqxx.
-        repeat eexists. eauto using corr_term_impl. }
-    have Hiso' : iso_heap
-      (fun l l'' => exists l',
-        (f' l l' \/ l = size H1' /\ l' = size H') /\
-        (f' l'' l' \/ l'' = size H1' /\ l' = size H'))
-      (rcons H1' (Some t5)) (rcons H1' (Some t5)).
-    { apply: (iso_heap_segment_dom (fun l l'' =>
-        (exists l', f' l l' /\ f' l'' l') \/
-        l = size H1' /\ l'' = size H1')).
-      - apply: iso_heap_segment_union => [ | ? ? [ -> -> ] ].
-        + apply: iso_heap_segment_rconsL.
-          apply: iso_heap_segment_rconsR.
-          apply: iso_heap_segment_cod; eauto.
-          move => ? ? [ ? [ ] ]. eauto.
-        + rewrite !nth_rcons !ltnn !eqxx.
-          repeat eexists.
-          apply: corr_term_impl.
-          * apply: corr_term_comp; eauto.
-            apply: corr_term_sym; eauto.
-          * move => ? ? [ ? [ ] ]. eauto 7.
-      - move => ? ? [ ? [ [ Hf | [ ? ? ] ] [ Hf' | [ ? ? ] ] ] ]; subst; eauto.
-        + move: (corr_heap_segment_boundR _ _ _ _ Hcorr0 _ _ Hf).
-          by rewrite ltnn.
-        + move: (corr_heap_segment_boundR _ _ _ _ Hcorr0 _ _ Hf').
-          by rewrite ltnn. }
-    move: (IHeval_need2 _ _ _ Hterm' Hcorr' Hiso') =>
-      [ ? [ ? [ ? [ ? [ ? [ ? [ ? ? ] ] ] ] ] ] ].
+  move => Hcorr Hcorr' Hdisj ? ? [ Hf | Hf' ];
+  [ move: (Hcorr _ _ Hf) | move: (Hcorr' _ _ Hf') ];
+  move => [ ? [ -> [ ? [ -> [ ? | [ ? [ ? [ ? [ ? [ ? [ ? Hcon ] ] ] ] ] ] ] ] ] ] ];
+  repeat (eexists; eauto); right; do 6 (eexists; eauto).
+  - move => ? [ /Hcon [ ? [ -> ? ] ] | /(Hdisj _ _ Hf) [ ] ].
     repeat (eexists; eauto).
-  - repeat (eexists; eauto).
-  - have Hterm' : corr_term
-      (fun l l' => f l l' \/
-        exists n, n < size ts0 /\ l = size H1 + n /\ l' = size H + n)
-      (subst (scat (mkseq (Loc \o addn (size H1)) (size ts0)) Var) t0)
-      (subst (scat (mkseq (Loc \o addn (size H)) (size ts)) Var) t).
-    { apply: corr_term_subst => [ | x ];
-      eauto using corr_term_impl.
-      rewrite !nth_scat H5.
-      case (leqP (size ts) x) => ?.
-      - by rewrite !nth_default ?size_mkseq.
-      - rewrite !nth_mkseq => /=; eauto 6. }
-    have Hcorr' : corr_heap
-      (fun l l' => f l l' \/
-        exists n, n < size ts0 /\ l = size H1 + n /\ l' = size H + n)
-      (H1 ++ map (@Some _ \o
-         subst (scat (mkseq (Loc \o addn (size H1)) (size ts0)) Var)) ts0)
-      (H ++ map (@Some _ \o
-         subst (scat (mkseq (Loc \o addn (size H)) (size ts)) Var)) ts).
-    { apply: corr_heap_segment_union.
-      - apply: corr_heap_segment_cod; eauto.
-        apply: corr_heap_catL.
-        by apply: corr_heap_segment_catR.
-      - apply: iso_heap_segment_corr_heap_segment => ? ? [ x [ ? [ -> -> ] ] ].
-        rewrite !nth_cat !ltnNge !leq_addr !addKn !(nth_map (Var 0)); try congruence.
-        repeat eexists.
-        apply: corr_term_subst => [ | y ];
-        eauto using corr_term_impl.
-        rewrite !nth_scat H5.
-        case (leqP (size ts) y) => ?.
-        + by rewrite !nth_default ?size_mkseq.
-        + rewrite !nth_mkseq => /=; eauto 6. }
-    have Hiso' : iso_heap
-      (fun l l'' => exists l',
-        (f l l' \/ exists n, n < size ts0 /\ l = size H1 + n /\ l' = size H + n) /\
-        (f l'' l' \/ exists n, n < size ts0 /\ l'' = size H1 + n /\ l' = size H + n))
-      (H1 ++ map (@Some _ \o
-         subst (scat (mkseq (Loc \o addn (size H1)) (size ts0)) Var)) ts0)
-      (H1 ++ map (@Some _ \o
-         subst (scat (mkseq (Loc \o addn (size H1)) (size ts0)) Var)) ts0).
-    { apply: (iso_heap_segment_dom (fun l l'' =>
-        (exists l', f l l' /\ f l'' l') \/
-        (exists n, n < size ts0 /\ l = size H1 + n /\ l'' = size H1 + n))).
-      - apply: iso_heap_segment_union => [ | ? ? [ x [ ? [ -> -> ] ] ] ].
-        + apply: iso_heap_segment_catL.
-          apply: iso_heap_segment_catR.
-          apply: iso_heap_segment_cod; eauto.
-          move => ? ? [ ? [ ] ]. eauto.
-        + rewrite !nth_cat !ltnNge !leq_addr !addKn !(nth_map (Var 0)); try congruence.
-          repeat eexists.
-          apply: corr_term_subst => [ | y ].
-          * apply: corr_term_comp; [ | apply: corr_term_sym ];
-            eauto using corr_term_impl.
-          * rewrite nth_scat.
-            { case (leqP (size ts0) y) => ?.
-              - by rewrite nth_default ?size_mkseq.
-              - rewrite !nth_mkseq => //=;
-                repeat (econstructor; eauto). }
-      - move => ? ? [ ? [ ] ]
-          [ Hf | [ ? [ ? [ ? ? ] ] ] ]
-          [ Hf' | [ ? [ ? [ ? Heq ] ] ] ]; subst; eauto.
-        + move: (corr_heap_segment_boundR _ _ _ _ Hcorr _ _ Hf).
-          by rewrite ltnNge leq_addr.
-        + move: (corr_heap_segment_boundR _ _ _ _ Hcorr _ _ Hf').
-          by rewrite ltnNge leq_addr.
-        + rewrite (addnI Heq). eauto. }
-    move: (IHeval_need _ _ _ Hterm' Hcorr' Hiso') =>
-      [ ? [ ? [ ? [ ? [ ? [ ? [ ? ? ] ] ] ] ] ] ].
+  - move => ? [ /Hdisj /(_ _ Hf') [ ] | /Hcon [ ? [ -> ? ] ] ].
     repeat (eexists; eauto).
 Qed.
 
-Theorem diverge_need_sound :
-  forall H2 t2,
-  diverge_need H2 t2 ->
-  forall f H1 t1,
-  corr_term f t1 t2 ->
-  corr_heap f H1 H2 ->
-  iso_heap (fun l1 l1' => exists l2, f l1 l2 /\ f l1' l2) H1 H1 ->
-  diverge_name H1 t1.
+Lemma corr_heap_iso_heap_comp R S H1 H2 H2' :
+  corr_heap R H1 H2 ->
+  iso_heap S H2 H2' ->
+  (forall l2 t2, nth None H2 l2 = Some t2 -> nth None H2' l2 = Some t2) ->
+  corr_heap (fun l1 l2' => R l1 l2' \/ exists l2, R l1 l2 /\ S l2 l2') H1 H2'.
 Proof.
-  cofix diverge_need_sound.
-  inversion 1; subst => [ f H1_ ? ];
-  inversion 1; subst => [ Hcorr Hiso ].
-  - move: (Hcorr _ _ H6) => [ ? [ ? [ ? [ ] ] ] ].
-    rewrite H1. inversion 1.
-    subst => [ [ Hterm | [ ? [ ? [ ? [ Hcbn [ ? [ ? Hterm ] ] ] ] ] ] ] ].
-    + econstructor; eauto.
-    + case: (value_diverge_need_disjoint _ _
-        (corr_term_valueL _ _ _ Hterm (eval_name_value _ _ _ _ Hcbn)) H3).
-  - apply: diverge_name_appL; eauto.
-  - move: (eval_need_sound _ _ _ _ H1 _ _ _ H7 Hcorr Hiso) =>
-      [ f' [ H1' [ ? [ ? [ Hcorr0 [ ? [ ] ] ] ] ] ] ].
-    inversion 1. subst => [ ? ].
-    have Hterm' : corr_term
-      (fun l l' => f' l l' \/ l = size H1' /\ l' = size H')
-      (subst (scons (Loc (size H1')) Var) t)
-      (subst (scons (Loc (size H')) Var) t0).
-    { apply: corr_term_subst => [ | [ | ? ] ] /=;
-      eauto using corr_term_impl. }
-    have Hcorr' : corr_heap
-      (fun l l' => f' l l' \/ l = size H1' /\ l' = size H')
-      (rcons H1' (Some t4)) (rcons H' (Some t3)).
-    { apply: corr_heap_segment_union.
-      - apply: corr_heap_segment_cod; eauto.
-        apply: corr_heap_rconsL.
-        by apply: corr_heap_segment_rconsR.
-      - apply: iso_heap_segment_corr_heap_segment => ? ? [ -> -> ].
-        rewrite !nth_rcons !ltnn !eqxx.
-        repeat eexists. eauto using corr_term_impl. }
-    have Hiso' : iso_heap
-      (fun l l'' => exists l',
-        (f' l l' \/ l = size H1' /\ l' = size H') /\
-        (f' l'' l' \/ l'' = size H1' /\ l' = size H'))
-      (rcons H1' (Some t4)) (rcons H1' (Some t4)).
-    { apply: (iso_heap_segment_dom (fun l l'' =>
-        (exists l', f' l l' /\ f' l'' l') \/
-        l = size H1' /\ l'' = size H1')).
-      - apply: iso_heap_segment_union => [ | ? ? [ -> -> ] ].
-        + apply: iso_heap_segment_rconsL.
-          apply: iso_heap_segment_rconsR.
-          apply: iso_heap_segment_cod; eauto.
-          move => ? ? [ ? [ ] ]. eauto.
-        + rewrite !nth_rcons !ltnn !eqxx.
-          repeat eexists.
-          apply: corr_term_impl.
-          * apply: corr_term_comp; eauto.
-            apply: corr_term_sym; eauto.
-          * move => ? ? [ ? [ ] ]. eauto 7.
-      - move => ? ? [ ? [ [ Hf | [ ? ? ] ] [ Hf' | [ ? ? ] ] ] ]; subst; eauto.
-        + move: (corr_heap_segment_boundR _ _ _ _ Hcorr0 _ _ Hf).
-          by rewrite ltnn.
-        + move: (corr_heap_segment_boundR _ _ _ _ Hcorr0 _ _ Hf').
-          by rewrite ltnn. }
-    apply: diverge_name_appabs; eauto.
-  - have Hterm' : corr_term
-      (fun l l' => f l l' \/
-        exists n, n < size ts0 /\ l = size H1_ + n /\ l' = size H2 + n)
-      (subst (scat (mkseq (Loc \o addn (size H1_)) (size ts0)) Var) t0)
-      (subst (scat (mkseq (Loc \o addn (size H2)) (size ts)) Var) t).
-    { apply: corr_term_subst => [ | x ];
-      eauto using corr_term_impl.
-      rewrite !nth_scat H5.
-      case (leqP (size ts) x) => ?.
-      - by rewrite !nth_default ?size_mkseq.
-      - rewrite !nth_mkseq => /=; eauto 6. }
-    have Hcorr' : corr_heap
-      (fun l l' => f l l' \/
-        exists n, n < size ts0 /\ l = size H1_ + n /\ l' = size H2 + n)
-      (H1_ ++ map (@Some _ \o
-         subst (scat (mkseq (Loc \o addn (size H1_)) (size ts0)) Var)) ts0)
-      (H2 ++ map (@Some _ \o
-         subst (scat (mkseq (Loc \o addn (size H2)) (size ts)) Var)) ts).
-    { apply: corr_heap_segment_union.
-      - apply: corr_heap_segment_cod; eauto.
-        apply: corr_heap_catL.
-        by apply: corr_heap_segment_catR.
-      - apply: iso_heap_segment_corr_heap_segment => ? ? [ x [ ? [ -> -> ] ] ].
-        rewrite !nth_cat !ltnNge !leq_addr !addKn !(nth_map (Var 0)); try congruence.
-        repeat eexists. 
-        apply: corr_term_subst => [ | y ];
-        eauto using corr_term_impl.
-        rewrite !nth_scat H5.
-        case (leqP (size ts) y) => ?.
-        + by rewrite !nth_default ?size_mkseq.
-        + rewrite !nth_mkseq => /=; eauto 6. }
-    have Hiso' : iso_heap
-      (fun l l'' => exists l',
-        (f l l' \/ exists n, n < size ts0 /\ l = size H1_ + n /\ l' = size H2 + n) /\
-        (f l'' l' \/ exists n, n < size ts0 /\ l'' = size H1_ + n /\ l' = size H2 + n))
-      (H1_ ++ map (@Some _ \o
-         subst (scat (mkseq (Loc \o addn (size H1_)) (size ts0)) Var)) ts0)
-      (H1_ ++ map (@Some _ \o
-         subst (scat (mkseq (Loc \o addn (size H1_)) (size ts0)) Var)) ts0).
-    { apply: (iso_heap_segment_dom (fun l l'' =>
-        (exists l', f l l' /\ f l'' l') \/
-        (exists n, n < size ts0 /\ l = size H1_ + n /\ l'' = size H1_ + n))).
-      - apply: iso_heap_segment_union => [ | ? ? [ x [ ? [ -> -> ] ] ] ].
-        + apply: iso_heap_segment_catL.
-          apply: iso_heap_segment_catR.
-          apply: iso_heap_segment_cod; eauto.
-          move => ? ? [ ? [ ] ]. eauto.
-        + rewrite !nth_cat !ltnNge !leq_addr !addKn !(nth_map (Var 0)); try congruence.
-          repeat eexists.
-          apply: corr_term_subst => [ | y ].
-          * apply: corr_term_comp; [ | apply: corr_term_sym ];
-            eauto using corr_term_impl.
-          * rewrite nth_scat.
-            { case (leqP (size ts0) y) => ?.
-              - by rewrite nth_default ?size_mkseq.
-              - rewrite !nth_mkseq => //=;
-                repeat (econstructor; eauto). }
-      - move => ? ? [ ? [ ] ]
-          [ Hf | [ ? [ ? [ ? ? ] ] ] ]
-          [ Hf' | [ ? [ ? [ ? Heq ] ] ] ]; subst; eauto.
-        + move: (corr_heap_segment_boundR _ _ _ _ Hcorr _ _ Hf).
-          by rewrite ltnNge leq_addr.
-        + move: (corr_heap_segment_boundR _ _ _ _ Hcorr _ _ Hf').
-          by rewrite ltnNge leq_addr.
-        + rewrite (addnI Heq). eauto. }
-    apply: diverge_name_let. eauto.
+  move => Hcorr Hiso Hsur.
+  have Hiso' : iso_heap (fun l2 l2' => S l2 l2' \/ l2 = l2' /\ exists l1, R l1 l2) H2 H2'.
+  { apply: iso_heap_segment_union; apply: iso_heap_segment_cod.
+    - exact: Hiso.
+    - eauto.
+    - apply: iso_heap_segment_extR.
+      + apply: iso_heap_segment_refl.
+        apply: corr_heap_segment_wf_heap_segmentR; eauto.
+      + eauto.
+    - move => ? ? [ -> [ ] ]. eauto. }
+  apply (corr_heap_segment_dom (fun l1 l2' => exists l2, R l1 l2 /\ (S l2 l2' \/ l2 = l2' /\ exists l1, R l1 l2))).
+  - apply (corr_heap_segment_cod _ (fun l1 l2' => exists l2, R l1 l2 /\ (S l2 l2' \/ l2 = l2' /\ exists l1, R l1 l2))).
+    { move => ? ? [ ? [ ] ]
+        /Hcorr [ ? [ -> [ ? [ Hnth
+          [ Hterm | [ ? [ ? [ Hcbn [ ? [ Hiso'' [ Hterm Hcon ] ] ] ] ] ] ] ] ] ] ]
+        /Hiso' [ ? [ Hnth' [ ? [ -> Hterm' ] ] ] ];
+      move: Hnth Hnth' => ->; inversion 1; subst;
+      repeat eexists.
+      - eauto using corr_term_comp.
+      - right.
+        move: (eval_name_iso_heap _ _ _ _ Hcbn _ _ _ Hterm' Hiso') =>
+          [ ? [ ? [ ? [ ? [ ? [ ? ? ] ] ] ] ] ].
+        do 5 (eexists; eauto).
+        { apply: iso_heap_segment_comp; eauto.
+          apply: iso_heap_segment_comp.
+          - apply: iso_heap_segment_sym. eauto.
+          - apply: iso_heap_segment_union; apply: iso_heap_segment_cod.
+            + exact: Hiso''.
+            + auto.
+            + apply: iso_heap_segment_extR.
+              * apply: iso_heap_segment_refl.
+                apply: corr_heap_segment_wf_heap_segmentR. eauto.
+              * move => ? ? ?. apply: eval_name_heap. eauto.
+            + eauto. }
+        split.
+        { apply: corr_term_impl.
+          - apply: corr_term_comp; eauto.
+          - move => ? ? [ ? [ [ ? | [ ? [ ? ? ] ] ] ? ] ];
+            right; repeat (eexists; eauto). }
+        move => ? [ ? [ ] ]
+          /Hcon [ ? [ Hnth'' ? ] ]
+          /Hiso' [ ? [ Hnth''' [ ? [ -> ? ] ] ] ].
+        move: Hnth'' Hnth''' => ->. inversion 1. subst.
+        repeat (eexists; eauto).
+        { apply: corr_term_impl.
+          - apply: corr_term_comp; eauto.
+            apply: corr_term_comp; eauto.
+            apply: corr_term_sym. eauto.
+          - move => ? ? [ ? [ [ ? [ ? [ ? [ ? ? ] ] ] ] ? ] ].
+            repeat (eexists; eauto). } }
+    move => ? ? [ ? [ ? [ ? | [ <- [ ? ? ] ] ] ] ]; eauto.
+  - move => ? ? [ ? | [ ? [ ? ? ] ] ]; repeat (eexists; eauto).
 Qed.
 
-Theorem eval_need_complete H1 t1 H1' v1 :
-  eval_name H1 t1 H1' v1 ->
+Corollary corr_heap_extR R H1 H2 H2' :
+  corr_heap R H1 H2 ->
+  ( forall l2 t,
+    nth None H2 l2 = Some t ->
+    nth None H2' l2 = Some t ) ->
+  corr_heap R H1 H2'.
+Proof.
+  move => Hcorr Hext.
+  apply: corr_heap_segment_dom.
+  - apply: corr_heap_segment_cod.
+    + apply: corr_heap_iso_heap_comp; eauto.
+      apply: iso_heap_segment_extR.
+      * apply: iso_heap_segment_refl.
+        apply: corr_heap_segment_wf_heap_segmentR; eauto.
+      * move => ? ? [ -> [ ] ]. eauto.
+    + move => ? ? [ ? | [ ? [ ? [ <- ] ] ] ]; eauto.
+  - move => /=. eauto.
+Qed.
+
+Corollary corr_heap_catR f H1 H2 Hd :
+  corr_heap f H1 H2 ->
+  corr_heap f H1 (H2 ++ Hd).
+Proof.
+  move => /corr_heap_extR.
+  apply => l' ?.
+  by move: nth_cat (leqP (size H2) l') => -> [ /(nth_default _) -> | ].
+Qed.
+
+Corollary corr_heap_rconsR f H1 H2 o :
+  corr_heap f H1 H2 ->
+  corr_heap f H1 (rcons H2 o).
+Proof. by rewrite -cats1 => /corr_heap_catR. Qed.
+
+Theorem eval_need_sound H1 t1 H1' v1 :
+  eval_need H1 t1 H1' v1 ->
   forall f H2 t2,
   corr_term f t1 t2 ->
   corr_heap f H1 H2 ->
-  iso_heap (fun l1 l1' => exists l2, f l1 l2 /\ f l1' l2) H1 H1 ->
   exists f' H2' v2,
-  eval_need H2 t2 H2' v2 /\
+  eval_name H2 t2 H2' v2 /\
   corr_heap f' H1' H2' /\
-  iso_heap (fun l1 l1' => exists l2, f' l1 l2 /\ f' l1' l2) H1' H1' /\
   corr_term f' v1 v2 /\
   (forall l1 l2, f l1 l2 -> f' l1 l2).
 Proof.
-  induction 1; inversion 1; subst => [ Hcorr Hiso ].
+  induction 1; inversion 1; subst => [ Hcorr ].
   - move: (Hcorr _ _ H5) => [ ? [ ] ].
     rewrite H0. inversion 1.
-    subst => [ [ ? [ Hnth [ Hterm | [ ? [ H1' [ ? [ Hcbn [ g [ ? Hterm' ] ] ] ] ] ] ] ] ] ].
-    + move: (IHeval_name _ _ _ Hterm Hcorr Hiso) =>
-        [ f' [ ? [ ? [ Hcbn [ Hcorr' [ Hiso' [ ? Himpl ] ] ] ] ] ] ].
+    subst => [ [ ? [ Hnth [ Hterm | [ H2' [ ? [ Hcbn [ g [ ? [ Hterm' ? ] ] ] ] ] ] ] ] ] ].
+    + move: (IHeval_need _ _ _ Hterm Hcorr) =>
+        [ f' [ ? [ ? [ Hcbn [ Hcorr' [ ? Himpl ] ] ] ] ] ].
       do 5 (eexists; eauto).
-      apply (corr_heap_segment_dom (fun l l0' => l0' != l' /\ f' l l0' \/ l0' = l' /\ f' l l0')).
+      apply (corr_heap_segment_dom (fun l1 l2 => l1 != l /\ f' l1 l2 \/ l1 = l /\ f' l1 l2)).
       { apply: corr_heap_segment_union.
-        - apply: corr_heap_segment_extR.
+        - apply: corr_heap_segment_extL.
           + apply: corr_heap_segment_dom; eauto.
             by move => ? ? [ ].
           + move => ? ? [ /negPf Hneq ? ] ?.
@@ -625,104 +355,64 @@ Proof.
             by rewrite Hneq.
         - move => ? ? [ ? ] Hf'. subst.
           rewrite nth_set_nth => /=.
+          have Hiso := corr_heap_segment_iso_heap_segmentR _ _ _ _ Hcorr.
+          have Hiso' := corr_heap_segment_iso_heap_segmentR _ _ _ _ Hcorr'.
           move: (Hiso' _ _ (ex_intro _ _ (conj Hf' (Himpl _ _ H5)))) =>
-            [ ? [ -> [ ? [ ] ] ] ].
-          rewrite (eval_name_heap _ _ _ _ H1 _ _ H0) eqxx.
+            [ ? [ Hnth' [ ? [ ] ] ] ].
+          rewrite Hnth' (eval_name_heap _ _ _ _ Hcbn _ _ Hnth) eqxx.
           inversion 1. subst => [ Hterm' ].
-          repeat eexists. right. split.
-          + apply: wf_term_impl.
-            * apply: corr_term_wf_termL; eauto.
-            * move => ? [ ? [ ? [ ] ] ]. eauto.
-          + move: (eval_name_iso_heap _ _ _ _ H1 _ _ _
-              (corr_term_comp _ _ _ _ Hterm' _
-                (corr_term_comp _ _ _ _ Hterm _ (corr_term_sym _ _ _ Hterm)))
-              (iso_heap_segment_comp _ _ _ _ _ _ _ Hiso'
-                (iso_heap_segment_extL _ _ _ _ _ Hiso
-                  (fun _ _ _ => eval_name_heap _ _ _ _ H1 _)))) =>
-              [ ? [ ? [ ? [ ? [ ? [ ? ? ] ] ] ] ] ].
-            repeat (eexists; eauto using corr_term_comp). }
-      move => ? l'0.
-      case (@eqP _ l'0 l') => /= [ -> | ]; eauto.
-    + move: (eval_name_det _ _ _ _ H1 _ _ Hcbn)
-        (value_eval_need H2 _
-          (corr_term_valueL _ _ _ Hterm' (eval_name_value _ _ _ _ Hcbn))) => [ ? ? ] ?. subst.
-      have Hiso' : iso_heap (fun l l' => g l l' \/ l = l' /\ exists l', f l l') H1' H.
-      { apply: iso_heap_segment_union.
-        - apply: iso_heap_segment_cod; eauto.
-        - apply: iso_heap_segment_extL.
-          + apply: iso_heap_segment_cod.
-            * apply: iso_heap_segment_refl.
-              apply: corr_heap_segment_wf_heap_segmentL. eauto.
-            * eauto.
-          + move => ? ? ?. apply: eval_name_heap. eauto. }
+          repeat eexists. right.
+          move: (eval_name_iso_heap _ _ _ _ Hcbn _ _ _
+            (corr_term_comp _ _ _ _
+              (corr_term_comp _ _ _ _ (corr_term_sym _ _ _ Hterm) _ Hterm) _
+              (corr_term_sym _ _ _ Hterm'))
+            (iso_heap_segment_comp _ _ _ _ _ _ _ 
+              (iso_heap_segment_extR _ _ _ _ _ Hiso
+                (fun _ _ _ => eval_name_heap _ _ _ _ Hcbn _))
+              (iso_heap_segment_sym _ _ _ _ Hiso'))) =>
+          [ ? [ ? [ ? [ ? [ ? [ ? ? ] ] ] ] ] ].
+          do 6 (eexists; eauto).
+          + apply: corr_term_impl.
+            * apply: corr_term_comp; eauto.
+            * move => //=. eauto.
+          + move => ? [ ? Hf ].
+            move: (Hiso' _ _ (ex_intro _ _ (conj Hf' Hf))) => [ ? [ ] ].
+            rewrite Hnth'. inversion 1. subst. eauto.
+        - move => ? ? [ /eqP ? ? ] ? [ ]. eauto. }
+      move => l1 l2.
+      case (@eqP _ l1 l) => /= [ -> | ]; eauto.
+    + case: (eval_need_det _ _ _ _ H1 _ _
+        (value_eval_need _ _
+          (corr_term_valueR _ _ _ Hterm' (eval_name_value _ _ _ _ Hcbn)))) => ? ?. subst.
       do 5 (eexists; eauto).
-      { apply: (iso_heap_corr_heap_segment_comp _ f f _ _ _ Hiso'); eauto.
-        apply: (corr_heap_segment_extR _ _ _ _ _ Hcorr) => ? l'0 ? ?.
-        move: nth_set_nth (@eqP _ l'0 l') => -> /= [ ? | // ].
-        subst. by rewrite Hnth. }
-      split.
-      { apply: iso_heap_segment_dom.
-        - apply: iso_heap_segment_cod.
-          + apply: iso_heap_segment_comp; eauto.
-            apply: iso_heap_segment_sym.
-            apply: iso_heap_segment_comp; eauto.
-          + move => ? ?
-              [ ? [ ] ] [ ? | [ -> [ ? ? ] ] ]
-              [ ? [ ] ] [ ? | [ -> [ ? ? ] ] ] [ ? [ ? ? ] ];
-            repeat (eexists; eauto).
-        - move => ? ? [ ? [ ] ]
-            [ ? [ ] ] [ ? | [ -> [ ? ? ] ] ] ?
-            [ ? [ ] ] [ ? | [ -> [ ? ? ] ] ] ?;
-          repeat (rewrite -?plus_n_O; eexists; eauto). }
-      split.
-      { apply: corr_term_impl; eauto.
-        move => ? ? [ ? [ ] ]. eauto. }
-      eauto 6.
-  - move: (IHeval_name1 _ _ _ H6 Hcorr Hiso) =>
-      [ f' [ H2' [ ? [ ? [ Hcorr0 [ ? [ ] ] ] ] ] ] ].
+      { apply: corr_heap_iso_heap_comp; eauto.
+        apply: (corr_heap_segment_extL _ _ _ _ _ Hcorr) => l1 ? ? ?.
+        move: nth_set_nth (@eqP _ l1 l) => -> /= [ ? | // ].
+        subst. by rewrite H0. }
+      eauto.
+  - move: (IHeval_need1 _ _ _ H6 Hcorr) =>
+      [ f' [ H2' [ ? [ ? [ Hcorr0 [ ] ] ] ] ] ].
     inversion 1. subst => [ ? ].
     have Hterm' : corr_term
       (fun l l' => f' l l' \/ l = size H' /\ l' = size H2')
       (subst (scons (Loc (size H')) Var) t0)
       (subst (scons (Loc (size H2')) Var) t').
-    { apply: corr_term_subst => [ | [ | ? ] /= ];
+    { apply: corr_term_subst => [ | [ | ? ] ] /=;
       eauto using corr_term_impl. }
     have Hcorr' : corr_heap
       (fun l l' => f' l l' \/ l = size H' /\ l' = size H2')
       (rcons H' (Some t2)) (rcons H2' (Some t2')).
     { apply: corr_heap_segment_union.
       - apply: corr_heap_segment_cod; eauto.
-        apply: corr_heap_rconsL.
-        by apply: corr_heap_segment_rconsR.
+        apply: corr_heap_segment_rconsL.
+        by apply: corr_heap_rconsR.
       - apply: iso_heap_segment_corr_heap_segment => ? ? [ -> -> ].
         rewrite !nth_rcons !ltnn !eqxx.
-        repeat eexists. eauto using corr_term_impl. }
-    have Hiso' : iso_heap
-      (fun l l'' => exists l',
-        (f' l l' \/ l = size H' /\ l' = size H2') /\
-        (f' l'' l' \/ l'' = size H' /\ l' = size H2'))
-      (rcons H' (Some t2)) (rcons H' (Some t2)).
-    { apply: (iso_heap_segment_dom (fun l l'' =>
-        (exists l', f' l l' /\ f' l'' l') \/
-        l = size H' /\ l'' = size H')).
-      - apply: iso_heap_segment_union => [ | ? ? [ -> -> ] ].
-        + apply: iso_heap_segment_rconsL.
-          apply: iso_heap_segment_rconsR.
-          apply: iso_heap_segment_cod; eauto.
-          move => ? ? [ ? [ ] ]. eauto.
-        + rewrite !nth_rcons !ltnn !eqxx.
-          repeat eexists.
-          apply: corr_term_impl.
-          * apply: corr_term_comp; eauto.
-            apply: corr_term_sym; eauto.
-          * move => ? ? [ ? [ ] ]. eauto 7.
-      - move => ? ? [ ? [ [ Hf | [ ? ? ] ] [ Hf' | [ ? ? ] ] ] ]; subst; eauto.
-        + move: (corr_heap_segment_boundR _ _ _ _ Hcorr0 _ _ Hf).
-          by rewrite ltnn.
-        + move: (corr_heap_segment_boundR _ _ _ _ Hcorr0 _ _ Hf').
-          by rewrite ltnn. }
-    move: (IHeval_name2 _ _ _ Hterm' Hcorr' Hiso') =>
-      [ ? [ ? [ ? [ ? [ ? [ ? [ ? ? ] ] ] ] ] ] ].
+        repeat eexists. eauto using corr_term_impl.
+      - move => ? ? Hf' ? [ ? ? ]. subst.
+        by move: ltnn (corr_heap_segment_boundL _ _ _ _ Hcorr0 _ _ Hf') => ->. }
+    move: (IHeval_need2 _ _ _ Hterm' Hcorr') =>
+      [ ? [ ? [ ? [ ? [ ? [ ? ? ] ] ] ] ] ].
     repeat (eexists; eauto).
   - repeat (eexists; eauto).
   - have Hterm' : corr_term
@@ -745,8 +435,8 @@ Proof.
          subst (scat (mkseq (Loc \o addn (size H2)) (size ts')) Var)) ts').
     { apply: corr_heap_segment_union.
       - apply: corr_heap_segment_cod; eauto.
-        apply: corr_heap_catL.
-        by apply: corr_heap_segment_catR.
+        apply: corr_heap_segment_catL.
+        by apply: corr_heap_catR.
       - apply: iso_heap_segment_corr_heap_segment => ? ? [ x [ ? [ -> -> ] ] ].
         rewrite !nth_cat !ltnNge !leq_addr !addKn !(nth_map (Var 0)); try congruence.
         repeat eexists.
@@ -755,108 +445,55 @@ Proof.
         rewrite !nth_scat H5.
         case (leqP (size ts') y) => ?.
         + by rewrite !nth_default ?size_mkseq.
-        + rewrite !nth_mkseq => /=; eauto 6. }
-    have Hiso' : iso_heap
-      (fun l l'' => exists l',
-        (f l l' \/ exists n, n < size ts /\ l = size H + n /\ l' = size H2 + n) /\
-        (f l'' l' \/ exists n, n < size ts /\ l'' = size H + n /\ l' = size H2 + n))
-      (H ++ map (@Some _ \o
-         subst (scat (mkseq (Loc \o addn (size H)) (size ts)) Var)) ts)
-      (H ++ map (@Some _ \o
-         subst (scat (mkseq (Loc \o addn (size H)) (size ts)) Var)) ts).
-    { apply: (iso_heap_segment_dom (fun l l'' =>
-        (exists l', f l l' /\ f l'' l') \/
-        (exists n, n < size ts /\ l = size H + n /\ l'' = size H + n))).
-      - apply: iso_heap_segment_union => [ | ? ? [ x [ ? [ -> -> ] ] ] ].
-        + apply: iso_heap_segment_catL.
-          apply: iso_heap_segment_catR.
-          apply: iso_heap_segment_cod; eauto.
-          move => ? ? [ ? [ ] ]. eauto.
-        + rewrite !nth_cat !ltnNge !leq_addr !addKn !(nth_map (Var 0)); try congruence.
-          repeat eexists.
-          apply: corr_term_subst => [ | y ].
-          * apply: corr_term_comp; [ | apply: corr_term_sym ];
-            eauto using corr_term_impl.
-          * rewrite nth_scat.
-            { case (leqP (size ts) y) => ?.
-              - by rewrite nth_default ?size_mkseq.
-              - rewrite !nth_mkseq => //=;
-                repeat (econstructor; eauto). }
-      - move => ? ? [ ? [ ] ]
-          [ Hf | [ ? [ ? [ ? ? ] ] ] ]
-          [ Hf' | [ ? [ ? [ ? Heq ] ] ] ]; subst; eauto.
-        + move: (corr_heap_segment_boundR _ _ _ _ Hcorr _ _ Hf).
-          by rewrite ltnNge leq_addr.
-        + move: (corr_heap_segment_boundR _ _ _ _ Hcorr _ _ Hf').
-          by rewrite ltnNge leq_addr.
-        + rewrite (addnI Heq). eauto. }
-    move: (IHeval_name _ _ _ Hterm' Hcorr' Hiso') =>
-      [ ? [ ? [ ? [ ? [ ? [ ? [ ? ? ] ] ] ] ] ] ].
+        + rewrite !nth_mkseq => /=; eauto 6.
+      - move => ? ? Hf ? [ ? [ ? [ ? ? ] ] ]. subst.
+        move: (corr_heap_segment_boundL _ _ _ _ Hcorr _ _ Hf).
+        by rewrite ltnNge leq_addr. }
+    move: (IHeval_need _ _ _ Hterm' Hcorr') =>
+      [ ? [ ? [ ? [ ? [ ? [ ? ? ] ] ] ] ] ].
     repeat (eexists; eauto).
 Qed.
 
-Theorem diverge_need_complete :
+Theorem diverge_need_sound :
   forall H1 t1,
-  diverge_name H1 t1 ->
+  diverge_need H1 t1 ->
   forall f H2 t2,
   corr_term f t1 t2 ->
   corr_heap f H1 H2 ->
-  iso_heap (fun l1 l1' => exists l2, f l1 l2 /\ f l1' l2) H1 H1 ->
-  diverge_need H2 t2.
+  diverge_name H2 t2.
 Proof.
-  cofix diverge_need_complete.
+  cofix diverge_need_sound.
   inversion 1; subst => [ f H2_ ? ];
-  inversion 1; subst => [ Hcorr Hiso ].
+  inversion 1; subst => [ Hcorr ].
   - move: (Hcorr _ _ H5) => [ ? [ ] ].
     rewrite H2. inversion 1.
-    subst => [ [ ? [ ? [ Hterm | [ ? [ ? [ ? [ Hcbn [ ? [ ? Hterm ] ] ] ] ] ] ] ] ] ].
+    subst => [ [ ? [ ? [ Hterm | [ ? [ ? [ Hcbn [ ? [ ? [ Hterm ? ] ] ] ] ] ] ] ] ] ].
     + econstructor; eauto.
-    + case: (eval_name_diverge_name_disjoint _ _ _ _ Hcbn H3).
-  - apply: diverge_need_appL; eauto.
-  - move: (eval_need_complete _ _ _ _ H2 _ _ _ H6 Hcorr Hiso) =>
-      [ f' [ H2' [ ? [ ? [ Hcorr0 [ ? [ ] ] ] ] ] ] ].
+    + case: (value_diverge_need_disjoint _ _
+        (corr_term_valueR _ _ _ Hterm (eval_name_value _ _ _ _ Hcbn)) H3).
+  - apply: diverge_name_appL; eauto.
+  - move: (eval_need_sound _ _ _ _ H2 _ _ _ H6 Hcorr) =>
+      [ f' [ H2' [ ? [ ? [ Hcorr0 [ ] ] ] ] ] ].
     inversion 1. subst => [ ? ].
     have Hterm' : corr_term
       (fun l l' => f' l l' \/ l = size H' /\ l' = size H2')
       (subst (scons (Loc (size H')) Var) t0)
       (subst (scons (Loc (size H2')) Var) t').
-    { apply: corr_term_subst => [ | [ | ? ] /= ];
+    { apply: corr_term_subst => [ | [ | ? ] ] /=;
       eauto using corr_term_impl. }
     have Hcorr' : corr_heap
       (fun l l' => f' l l' \/ l = size H' /\ l' = size H2')
       (rcons H' (Some t3)) (rcons H2' (Some t2')).
     { apply: corr_heap_segment_union.
       - apply: corr_heap_segment_cod; eauto.
-        apply: corr_heap_rconsL.
-        by apply: corr_heap_segment_rconsR.
+        apply: corr_heap_segment_rconsL.
+        by apply: corr_heap_rconsR.
       - apply: iso_heap_segment_corr_heap_segment => ? ? [ -> -> ].
         rewrite !nth_rcons !ltnn !eqxx.
-        repeat eexists. eauto using corr_term_impl. }
-    have Hiso' : iso_heap
-      (fun l l'' => exists l',
-        (f' l l' \/ l = size H' /\ l' = size H2') /\
-        (f' l'' l' \/ l'' = size H' /\ l' = size H2'))
-      (rcons H' (Some t3)) (rcons H' (Some t3)).
-    { apply: (iso_heap_segment_dom (fun l l'' =>
-        (exists l', f' l l' /\ f' l'' l') \/
-        l = size H' /\ l'' = size H')).
-      - apply: iso_heap_segment_union => [ | ? ? [ -> -> ] ].
-        + apply: iso_heap_segment_rconsL.
-          apply: iso_heap_segment_rconsR.
-          apply: iso_heap_segment_cod; eauto.
-          move => ? ? [ ? [ ] ]. eauto.
-        + rewrite !nth_rcons !ltnn !eqxx.
-          repeat eexists.
-          apply: corr_term_impl.
-          * apply: corr_term_comp; eauto.
-            apply: corr_term_sym; eauto.
-          * move => ? ? [ ? [ ] ]. eauto 7.
-      - move => ? ? [ ? [ [ Hf | [ ? ? ] ] [ Hf' | [ ? ? ] ] ] ]; subst; eauto.
-        + move: (corr_heap_segment_boundR _ _ _ _ Hcorr0 _ _ Hf).
-          by rewrite ltnn.
-        + move: (corr_heap_segment_boundR _ _ _ _ Hcorr0 _ _ Hf').
-          by rewrite ltnn. }
-    apply: diverge_need_appabs; eauto.
+        repeat eexists. eauto using corr_term_impl.
+      - move => ? ? Hf' ? [ ? ? ]. subst.
+        by move: ltnn (corr_heap_segment_boundL _ _ _ _ Hcorr0 _ _ Hf') => ->. }
+    apply: diverge_name_appabs; eauto.
   - have Hterm' : corr_term
       (fun l l' => f l l' \/
         exists n, n < size ts /\ l = size H1 + n /\ l' = size H2_ + n)
@@ -877,50 +514,225 @@ Proof.
          subst (scat (mkseq (Loc \o addn (size H2_)) (size ts')) Var)) ts').
     { apply: corr_heap_segment_union.
       - apply: corr_heap_segment_cod; eauto.
-        apply: corr_heap_catL.
-        by apply: corr_heap_segment_catR.
+        apply: corr_heap_segment_catL.
+        by apply: corr_heap_catR.
+      - apply: iso_heap_segment_corr_heap_segment => ? ? [ x [ ? [ -> -> ] ] ].
+        rewrite !nth_cat !ltnNge !leq_addr !addKn !(nth_map (Var 0)); try congruence.
+        repeat eexists. 
+        apply: corr_term_subst => [ | y ];
+        eauto using corr_term_impl.
+        rewrite !nth_scat H5.
+        case (leqP (size ts') y) => ?.
+        + by rewrite !nth_default ?size_mkseq.
+        + rewrite !nth_mkseq => /=; eauto 6.
+      - move => ? ? Hf ? [ ? [ ? [ ? ? ] ] ]. subst.
+        move: (corr_heap_segment_boundL _ _ _ _ Hcorr _ _ Hf).
+        by rewrite ltnNge leq_addr. }
+    apply: diverge_name_let. eauto.
+Qed.
+
+Theorem eval_need_complete H2 t2 H2' v2 :
+  eval_name H2 t2 H2' v2 ->
+  forall f H1 t1,
+  corr_term f t1 t2 ->
+  corr_heap f H1 H2 ->
+  exists f' H1' v1,
+  eval_need H1 t1 H1' v1 /\
+  corr_heap f' H1' H2' /\
+  corr_term f' v1 v2 /\
+  (forall l1 l2, f l1 l2 -> f' l1 l2).
+Proof.
+  induction 1; inversion 1; subst => [ Hcorr ].
+  - move: (Hcorr _ _ H6) => [ ? [ Hnth [ ? [ ] ] ] ].
+    rewrite H0. inversion 1.
+    subst => [ [ Hterm | [ H2' [ ? [ Hcbn [ g [ ? [ Hterm' ? ] ] ] ] ] ] ] ].
+    + move: (IHeval_name _ _ _ Hterm Hcorr) =>
+        [ f' [ ? [ ? [ Hcbn [ Hcorr' [ ? Himpl ] ] ] ] ] ].
+      do 5 (eexists; eauto).
+      apply (corr_heap_segment_dom (fun l1 l2 => l1 != l0 /\ f' l1 l2 \/ l1 = l0 /\ f' l1 l2)).
+      { apply: corr_heap_segment_union.
+        - apply: corr_heap_segment_extL.
+          + apply: corr_heap_segment_dom; eauto.
+            by move => ? ? [ ].
+          + move => ? ? [ /negPf Hneq ? ] ?.
+            rewrite nth_set_nth => /=.
+            by rewrite Hneq.
+        - move => ? ? [ ? ] Hf'. subst.
+          rewrite nth_set_nth => /=.
+          have Hiso := corr_heap_segment_iso_heap_segmentR _ _ _ _ Hcorr.
+          have Hiso' := corr_heap_segment_iso_heap_segmentR _ _ _ _ Hcorr'.
+          move: (Hiso' _ _ (ex_intro _ _ (conj Hf' (Himpl _ _ H6)))) =>
+            [ ? [ Hnth' [ ? [ ] ] ] ].
+          rewrite Hnth' (eval_name_heap _ _ _ _ H1 _ _ H0) eqxx.
+          inversion 1. subst => [ Hterm' ].
+          repeat eexists. right.
+          move: (eval_name_iso_heap _ _ _ _ H1 _ _ _
+            (corr_term_comp _ _ _ _
+              (corr_term_comp _ _ _ _ (corr_term_sym _ _ _ Hterm) _ Hterm) _
+              (corr_term_sym _ _ _ Hterm'))
+            (iso_heap_segment_comp _ _ _ _ _ _ _ 
+              (iso_heap_segment_extR _ _ _ _ _ Hiso
+                (fun _ _ _ => eval_name_heap _ _ _ _ H1 _))
+              (iso_heap_segment_sym _ _ _ _ Hiso'))) =>
+          [ ? [ ? [ ? [ ? [ ? [ ? ? ] ] ] ] ] ].
+          do 6 (eexists; eauto).
+          + apply: corr_term_impl.
+            * apply: corr_term_comp; eauto.
+            * move => //=. eauto.
+          + move => ? [ ? Hf ].
+            move: (Hiso' _ _ (ex_intro _ _ (conj Hf' Hf))) => [ ? [ ] ].
+            rewrite Hnth'. inversion 1. subst. eauto.
+        - move => ? ? [ /eqP ? ? ] ? [ ]. eauto. }
+      move => l1 l2.
+      case (@eqP _ l1 l0) => /= [ -> | ]; eauto.
+    + case: (eval_name_det _ _ _ _ H1 _ _ Hcbn) => ? ?. subst.
+      do 4 (eexists; eauto).
+      { econstructor; eauto.
+        apply: value_eval_need.
+        apply: corr_term_valueR; eauto.
+        apply: eval_name_value. eauto. }
+      split.
+      { apply: corr_heap_iso_heap_comp; eauto.
+        apply: (corr_heap_segment_extL _ _ _ _ _ Hcorr) => l1 ? ? ?.
+        move: nth_set_nth (@eqP _ l1 l0) => -> /= [ ? | // ].
+        subst. by rewrite Hnth. }
+      eauto.
+  - move: (IHeval_name1 _ _ _ H7 Hcorr) =>
+      [ f' [ H1' [ ? [ ? [ Hcorr0 [ ] ] ] ] ] ].
+    inversion 1. subst => [ ? ].
+    have Hterm' : corr_term
+      (fun l l' => f' l l' \/ l = size H1' /\ l' = size H')
+      (subst (scons (Loc (size H1')) Var) t)
+      (subst (scons (Loc (size H')) Var) t0).
+    { apply: corr_term_subst => [ | [ | ? ] ] /=;
+      eauto using corr_term_impl. }
+    have Hcorr' : corr_heap
+      (fun l l' => f' l l' \/ l = size H1' /\ l' = size H')
+      (rcons H1' (Some t5)) (rcons H' (Some t2)).
+    { apply: corr_heap_segment_union.
+      - apply: corr_heap_segment_cod; eauto.
+        apply: corr_heap_segment_rconsL.
+        by apply: corr_heap_rconsR.
+      - apply: iso_heap_segment_corr_heap_segment => ? ? [ -> -> ].
+        rewrite !nth_rcons !ltnn !eqxx.
+        repeat eexists. eauto using corr_term_impl.
+      - move => ? ? Hf' ? [ ? ? ]. subst.
+        by move: ltnn (corr_heap_segment_boundL _ _ _ _ Hcorr0 _ _ Hf') => ->. }
+    move: (IHeval_name2 _ _ _ Hterm' Hcorr') =>
+      [ ? [ ? [ ? [ ? [ ? [ ? ? ] ] ] ] ] ].
+    repeat (eexists; eauto).
+  - repeat (eexists; eauto).
+  - have Hterm' : corr_term
+      (fun l l' => f l l' \/
+        exists n, n < size ts0 /\ l = size H1 + n /\ l' = size H + n)
+      (subst (scat (mkseq (Loc \o addn (size H1)) (size ts0)) Var) t0)
+      (subst (scat (mkseq (Loc \o addn (size H)) (size ts)) Var) t).
+    { apply: corr_term_subst => [ | x ];
+      eauto using corr_term_impl.
+      rewrite !nth_scat H5.
+      case (leqP (size ts) x) => ?.
+      - by rewrite !nth_default ?size_mkseq.
+      - rewrite !nth_mkseq => /=; eauto 6. }
+    have Hcorr' : corr_heap
+      (fun l l' => f l l' \/
+        exists n, n < size ts0 /\ l = size H1 + n /\ l' = size H + n)
+      (H1 ++ map (@Some _ \o
+         subst (scat (mkseq (Loc \o addn (size H1)) (size ts0)) Var)) ts0)
+      (H ++ map (@Some _ \o
+         subst (scat (mkseq (Loc \o addn (size H)) (size ts)) Var)) ts).
+    { apply: corr_heap_segment_union.
+      - apply: corr_heap_segment_cod; eauto.
+        apply: corr_heap_segment_catL.
+        by apply: corr_heap_catR.
       - apply: iso_heap_segment_corr_heap_segment => ? ? [ x [ ? [ -> -> ] ] ].
         rewrite !nth_cat !ltnNge !leq_addr !addKn !(nth_map (Var 0)); try congruence.
         repeat eexists.
         apply: corr_term_subst => [ | y ];
         eauto using corr_term_impl.
         rewrite !nth_scat H5.
-        case (leqP (size ts') y) => ?.
+        case (leqP (size ts) y) => ?.
         + by rewrite !nth_default ?size_mkseq.
-        + rewrite !nth_mkseq => /=; eauto 6. }
-    have Hiso' : iso_heap
-      (fun l l'' => exists l',
-        (f l l' \/ exists n, n < size ts /\ l = size H1 + n /\ l' = size H2_ + n) /\
-        (f l'' l' \/ exists n, n < size ts /\ l'' = size H1 + n /\ l' = size H2_ + n))
-      (H1 ++ map (@Some _ \o
-         subst (scat (mkseq (Loc \o addn (size H1)) (size ts)) Var)) ts)
-      (H1 ++ map (@Some _ \o
-         subst (scat (mkseq (Loc \o addn (size H1)) (size ts)) Var)) ts).
-    { apply: (iso_heap_segment_dom (fun l l'' =>
-        (exists l', f l l' /\ f l'' l') \/
-        (exists n, n < size ts /\ l = size H1 + n /\ l'' = size H1 + n))).
-      - apply: iso_heap_segment_union => [ | ? ? [ x [ ? [ -> -> ] ] ] ].
-        + apply: iso_heap_segment_catL.
-          apply: iso_heap_segment_catR.
-          apply: iso_heap_segment_cod; eauto.
-          move => ? ? [ ? [ ] ]. eauto.
-        + rewrite !nth_cat !ltnNge !leq_addr !addKn !(nth_map (Var 0)); try congruence.
-          repeat eexists.
-          apply: corr_term_subst => [ | y ].
-          * apply: corr_term_comp; [ | apply: corr_term_sym ];
-            eauto using corr_term_impl.
-          * rewrite nth_scat.
-            { case (leqP (size ts) y) => ?.
-              - by rewrite nth_default ?size_mkseq.
-              - rewrite !nth_mkseq => //=;
-                repeat (econstructor; eauto). }
-      - move => ? ? [ ? [ ] ]
-          [ Hf | [ ? [ ? [ ? ? ] ] ] ]
-          [ Hf' | [ ? [ ? [ ? Heq ] ] ] ]; subst; eauto.
-        + move: (corr_heap_segment_boundR _ _ _ _ Hcorr _ _ Hf).
-          by rewrite ltnNge leq_addr.
-        + move: (corr_heap_segment_boundR _ _ _ _ Hcorr _ _ Hf').
-          by rewrite ltnNge leq_addr.
-        + rewrite (addnI Heq). eauto. }
+        + rewrite !nth_mkseq => /=; eauto 6.
+      - move => ? ? Hf ? [ ? [ ? [ ? ? ] ] ]. subst.
+        move: (corr_heap_segment_boundL _ _ _ _ Hcorr _ _ Hf).
+        by rewrite ltnNge leq_addr. }
+    move: (IHeval_name _ _ _ Hterm' Hcorr') =>
+      [ ? [ ? [ ? [ ? [ ? [ ? ? ] ] ] ] ] ].
+    repeat (eexists; eauto).
+Qed.
+
+Theorem diverge_need_complete :
+  forall H2 t2,
+  diverge_name H2 t2 ->
+  forall f H1 t1,
+  corr_term f t1 t2 ->
+  corr_heap f H1 H2 ->
+  diverge_need H1 t1.
+Proof.
+  cofix diverge_need_complete.
+  inversion 1; subst => [ f H1_ ? ];
+  inversion 1; subst => [ Hcorr ].
+  - move: (Hcorr _ _ H6) => [ ? [ ? [ ? [ ] ] ] ].
+    rewrite H1. inversion 1.
+    subst => [ [ ? | [ ? [ ? [ Hcbn [ ? [ ? [ ? ? ] ] ] ] ] ] ] ].
+    + econstructor; eauto.
+    + case: (eval_name_diverge_name_disjoint _ _ _ _ Hcbn H3).
+  - apply: diverge_need_appL; eauto.
+  - move: (eval_need_complete _ _ _ _ H1 _ _ _ H7 Hcorr) =>
+      [ f' [ H1' [ ? [ ? [ Hcorr0 [ ] ] ] ] ] ].
+    inversion 1. subst => [ ? ].
+    have Hterm' : corr_term
+      (fun l l' => f' l l' \/ l = size H1' /\ l' = size H')
+      (subst (scons (Loc (size H1')) Var) t)
+      (subst (scons (Loc (size H')) Var) t0).
+    { apply: corr_term_subst => [ | [ | ? ] /= ];
+      eauto using corr_term_impl. }
+    have Hcorr' : corr_heap
+      (fun l l' => f' l l' \/ l = size H1' /\ l' = size H')
+      (rcons H1' (Some t4)) (rcons H' (Some t3)).
+    { apply: corr_heap_segment_union.
+      - apply: corr_heap_segment_cod; eauto.
+        apply: corr_heap_segment_rconsL.
+        by apply: corr_heap_rconsR.
+      - apply: iso_heap_segment_corr_heap_segment => ? ? [ -> -> ].
+        rewrite !nth_rcons !ltnn !eqxx.
+        repeat eexists. eauto using corr_term_impl.
+      - move => ? ? Hf' ? [ ? ? ]. subst.
+        by move: ltnn (corr_heap_segment_boundL _ _ _ _ Hcorr0 _ _ Hf') => ->. }
+    apply: diverge_need_appabs; eauto.
+  - have Hterm' : corr_term
+      (fun l l' => f l l' \/
+        exists n, n < size ts0 /\ l = size H1_ + n /\ l' = size H2 + n)
+      (subst (scat (mkseq (Loc \o addn (size H1_)) (size ts0)) Var) t0)
+      (subst (scat (mkseq (Loc \o addn (size H2)) (size ts)) Var) t).
+    { apply: corr_term_subst => [ | x ];
+      eauto using corr_term_impl.
+      rewrite !nth_scat H5.
+      case (leqP (size ts) x) => ?.
+      - by rewrite !nth_default ?size_mkseq.
+      - rewrite !nth_mkseq => /=; eauto 6. }
+    have Hcorr' : corr_heap
+      (fun l l' => f l l' \/
+        exists n, n < size ts0 /\ l = size H1_ + n /\ l' = size H2 + n)
+      (H1_ ++ map (@Some _ \o
+         subst (scat (mkseq (Loc \o addn (size H1_)) (size ts0)) Var)) ts0)
+      (H2 ++ map (@Some _ \o
+         subst (scat (mkseq (Loc \o addn (size H2)) (size ts)) Var)) ts).
+    { apply: corr_heap_segment_union.
+      - apply: corr_heap_segment_cod; eauto.
+        apply: corr_heap_segment_catL.
+        by apply: corr_heap_catR.
+      - apply: iso_heap_segment_corr_heap_segment => ? ? [ x [ ? [ -> -> ] ] ].
+        rewrite !nth_cat !ltnNge !leq_addr !addKn !(nth_map (Var 0)); try congruence.
+        repeat eexists.
+        apply: corr_term_subst => [ | y ];
+        eauto using corr_term_impl.
+        rewrite !nth_scat H5.
+        case (leqP (size ts) y) => ?.
+        + by rewrite !nth_default ?size_mkseq.
+        + rewrite !nth_mkseq => /=; eauto 6.
+      - move => ? ? Hf ? [ ? [ ? [ ? ? ] ] ]. subst.
+        move: (corr_heap_segment_boundL _ _ _ _ Hcorr _ _ Hf).
+        by rewrite ltnNge leq_addr. }
     apply: diverge_need_let. eauto.
 Qed.
